elaborate.v: Upstream {spec,elab}_{impl/entails}

theories/lang/cpp/specs/elaborate.v
@@ -7,6 +7,7 @@
 (** Functionality to elaborate specifications that are written to take
     operands (i.e. [val]) and convert them to take materialized values.
  *)
+Require Import iris.proofmode.proofmode.
 From bedrock.lang.cpp Require Import ast logic semantics.
 From bedrock.lang.cpp.specs Require Import cpp_specs wp_spec_compat.
 
@@ -53,4 +54,67 @@ Section with_cpp.
    *)
   Definition cpp_spec (ret : type) (ts : list type) (wpp : WpSpec_cpp_val) : WpSpec_cpp_ptr :=
     elaborate ret ts wpp nil.
+
+  (** Specification implications
+
+      NOTE: these can be strengthened to include extra information about well-typed values.
+            (this includes [valid_ptr] on `this` if it exists                                                                  )
+      NOTE: this should do the extra plumbing to avoid [K], though it isn't clear how to do this
+      NOTE: this can be strengthened with extra fancy updates.
+   *)
+  Definition spec_impl {A R} (Q P : WpSpec mpredI A R) : mpredI :=
+    ∀ (vs : list A) (K : R → mpred), P vs K -∗ Q vs K.
+
+  (* TODO: some upstream proper instances use [wpspec_entails], unify the uses.
+  TODO: we should flip [wpspec_relation] like we flipped [fs_entails] for the
+  same reason. *)
+  Definition spec_entails {A R} :=
+    flip (wpspec_relation (PROP := mpredI) bi_entails (ARGS := A) (RESULT := R)).
+
+  Lemma spec_entails_impl {A R} Q P :
+    (|-- @spec_impl A R P Q) ↔
+    spec_entails P Q.
+  Proof.
+    rewrite /spec_impl/wpspec_relation; split; intros H **; first iApply H.
+    iIntros (??). iApply H.
+  Qed.
+
+  Lemma elab_impl (Q P : WpSpec mpredI val val) ret ts :
+    spec_impl Q P |-- spec_impl (cpp_spec ret ts Q) (cpp_spec ret ts P).
+  Proof.
+    rewrite /spec_impl/wp_specD/cpp_spec.
+    assert (forall ps xs Ps Qs,
+               (∀ (vs : list val) (K : val → mpred), spec_internal P [] [] [] vs K -∗ spec_internal Q [] [] [] vs K) -∗
+               ∀ (vs : list ptr) (K : ptr → mpred),
+                 spec_internal (elaborate ret ts P ps) xs Ps Qs vs K -∗ spec_internal (elaborate ret ts Q ps) xs Ps Qs vs K).
+    { induction ts; simpl; intros.
+      { case_match; rewrite /wp_spec_bind/=.
+        { iIntros "H" (??) "[$ P]".
+          iRevert "P"; iApply list_sep_into_frame.
+          iApply "H". }
+        { iIntros "H" (??) "[$ P]".
+          iRevert "P"; iApply list_sep_into_frame.
+          iApply "H"; eauto. } }
+      { case_match; rewrite /wp_spec_bind/=.
+        { iIntros "H" (??) "P".
+          iDestruct "P" as (x) "P".
+          iExists x.
+          iDestruct (IHts with "H") as "H".
+          by iApply "H". }
+        { iIntros "H" (??) "P".
+          iDestruct "P" as (x y) "P".
+          iExists x, y.
+          iDestruct (IHts with "H") as "H".
+          by iApply "H". } } }
+    { eauto. }
+  Qed.
+
+  Lemma elab_entails (Q P : WpSpec mpredI val val) ret ts :
+    spec_entails Q P ->
+    spec_entails (cpp_spec ret ts Q) (cpp_spec ret ts P).
+  Proof. intros H%spec_entails_impl. iApply elab_impl. iApply H. Qed.
+
+  #[global] Instance cpp_spec_mono ret ts :
+    Proper (spec_entails ==> spec_entails) (cpp_spec ret ts).
+  Proof. intros ???. exact: elab_entails. Qed.
 End with_cpp.
